{
 "cells": [
  {
   "cell_type": "markdown",
   "id": "fa4d7cc8",
   "metadata": {},
   "source": [
    "Linear Algebra : (link) <br>\n",
    "<br>\n",
    "Main Theorem : Let $M$ be a partitioned matrix of the form $M = \\begin{bmatrix} A & B \\\\ C & D \\end{bmatrix}$ where $A$ and $D$ are square matrices\n",
    "- If $A$ is invertible, then $\\det (M) = \\det (A) \\det (D - C A^{-1} B)$ <br>\n",
    "- If $D$ is invertible, then $\\det (M) = \\det (A - B D^{-1} C) \\det (D) \\ \\ $ <br>"
   ]
  },
  {
   "cell_type": "markdown",
   "id": "a3c8444d",
   "metadata": {},
   "source": [
    "Theorem 1 : If $M = \\begin{bmatrix} A & 0 \\\\ 0 & I_p \\end{bmatrix}$ or $M = \\begin{bmatrix} I_p & 0 \\\\ 0 & A \\end{bmatrix}$, then $\\det (M) = \\det (A)$\n",
    "- If $M = \\begin{bmatrix} A & 0 \\\\ 0 & I_p \\end{bmatrix}$, then cofactor expansion $p$ columns from the **right** shows that $\\det (M) = \\det (A)$\n",
    "- If $M = \\begin{bmatrix} I_p & 0 \\\\ 0 & A \\end{bmatrix}$, then cofactor expansion $p$ columns from the **left**, shows that $\\det (M) = \\det (A)$"
   ]
  },
  {
   "cell_type": "markdown",
   "id": "85cfdf47",
   "metadata": {},
   "source": [
    "Theorem 2 : if $M = \\begin{bmatrix} A & B \\\\ 0 & D \\end{bmatrix}$ or $M = \\begin{bmatrix} A & 0 \\\\ C & D \\end{bmatrix}$ where $A$ is $p \\times p$ and $D$ is $q \\times q$, then $\\det (M) = \\det (A) \\det (D)$\n",
    "- If $M = \\begin{bmatrix} A & B \\\\ 0 & D \\end{bmatrix}$, we can check $\\begin{bmatrix} I_p & 0 \\\\ 0 & D \\end{bmatrix} \\begin{bmatrix} I_p & B \\\\ 0 & I_q \\end{bmatrix} \\begin{bmatrix} A & 0 \\\\ 0 & I_q \\end{bmatrix} = \\begin{bmatrix} A & B \\\\ 0 & D \\end{bmatrix}$\n",
    "  - By Theorem 1, $\\begin{vmatrix} I_p & 0 \\\\ 0 & D \\end{vmatrix} = \\det (D)$, and $\\begin{vmatrix} A & 0 \\\\ 0 & I_q \\end{vmatrix} = \\det (A)$\n",
    "  - And $\\begin{vmatrix} I_p & B \\\\ 0 & I_q \\end{vmatrix} = \\begin{vmatrix} I_q \\end{vmatrix} = 1$, which can show by cofactor expansion down a column from the left\n",
    "  - Therefore, $\\det (M) = \\det (D) \\cdot 1 \\cdot \\det (A) = \\det (A) \\det (D)$\n",
    "- If $M = \\begin{bmatrix} A & 0 \\\\ C & D \\end{bmatrix}$, we can check $\\begin{bmatrix} A & 0 \\\\ 0 & I_q \\end{bmatrix} \\begin{bmatrix} I_p & 0 \\\\ C & I_q \\end{bmatrix} \\begin{bmatrix} I_p & 0 \\\\ 0 & D \\end{bmatrix} = \\begin{bmatrix} A & 0 \\\\ C & D \\end{bmatrix}$\n",
    "  - By Theorem 1, $\\begin{vmatrix} A & 0 \\\\ 0 & I_q \\end{vmatrix} = \\det (A)$, and $\\begin{vmatrix} I_p & 0 \\\\ 0 & D \\end{vmatrix} = \\det (D)$\n",
    "  - And $\\begin{vmatrix} I_p & 0 \\\\ C & I_q \\end{vmatrix} = \\begin{vmatrix} I_p \\end{vmatrix} = 1$, which can show by cofactor expansion down a column from the right\n",
    "  - Therefore, $\\det (M) = \\det (D) \\cdot 1 \\cdot \\det (A) = \\det (A) \\det (D)$\n",
    "- Also, obviously, if $M = \\begin{bmatrix} A & 0 \\\\ 0 & D \\end{bmatrix}$, then $\\det (M) = \\det (A) \\det (D)$"
   ]
  },
  {
   "cell_type": "markdown",
   "id": "3e713781",
   "metadata": {},
   "source": [
    "Main Theorem proof\n",
    "- If $A$ is invertible, by LDU decomposition, $M = \\begin{bmatrix} A & B \\\\ C & D \\end{bmatrix} = \\begin{bmatrix} I_p & 0 \\\\ CA^{-1} & I_q \\end{bmatrix} \\begin{bmatrix} A & 0 \\\\ 0 & D - CA^{-1}B \\end{bmatrix} \\begin{bmatrix} I_p & A^{-1}B \\\\ 0 & I_q \\end{bmatrix}$\n",
    "  - By Theorem 2, $\\begin{vmatrix} I_p & 0 \\\\ CA^{-1} & I_q \\end{vmatrix} = 1$, $\\begin{vmatrix} I_p & A^{-1}B \\\\ 0 & I_q \\end{vmatrix} = 1$, and $\\begin{vmatrix} A & 0 \\\\ 0 & D - CA^{-1}B \\end{vmatrix} = \\det (A) \\det (D - CA^{-1}B)$\n",
    "  - Therefore $\\det M = 1 \\cdot \\det (A) \\det (D - CA^{-1}B) \\cdot 1 = \\det (A) \\det (D - CA^{-1}B)$\n",
    "- If $D$ is invertible, by LDU decomposition, $M = \\begin{bmatrix} A & B \\\\ C & D \\end{bmatrix} = \\begin{bmatrix} I_p & BD^{-1} \\\\ 0 & I_q \\end{bmatrix} \\begin{bmatrix} A - BD^{-1}C & 0 \\\\ 0 & D \\end{bmatrix} \\begin{bmatrix} I_p & 0 \\\\ D^{-1}C & I_q \\end{bmatrix}$\n",
    "  - By Theorem 2, $\\begin{vmatrix} I_p & BD^{-1} \\\\ 0 & I_q \\end{vmatrix} = 1$, $\\begin{vmatrix} I_p & 0 \\\\ D^{-1}C & I_q \\end{vmatrix} = 1$, and $\\begin{vmatrix} A - BD^{-1}C & 0 \\\\ 0 & D \\end{vmatrix} = \\det (A - BD^{-1}C) \\det (D) $\n",
    "  - Therefore $\\det M = 1 \\cdot \\det (A - BD^{-1}C) \\det (D) \\cdot 1 = \\det (A - BD^{-1}C) \\det (D)$"
   ]
  }
 ],
 "metadata": {
  "kernelspec": {
   "display_name": "Python 3 (ipykernel)",
   "language": "python",
   "name": "python3"
  },
  "language_info": {
   "codemirror_mode": {
    "name": "ipython",
    "version": 3
   },
   "file_extension": ".py",
   "mimetype": "text/x-python",
   "name": "python",
   "nbconvert_exporter": "python",
   "pygments_lexer": "ipython3",
   "version": "3.10.2"
  }
 },
 "nbformat": 4,
 "nbformat_minor": 5
}
